{
 "cells": [
  {
   "cell_type": "markdown",
   "id": "8d64cd75-4148-4b33-b383-d1bf3796e013",
   "metadata": {},
   "source": [
    "### **Problems**\n",
    "\n",
    "For $$ g(z) = \\frac{z+3}{(z+1)^2} $$ evaluate,\n",
    "\n",
    "(a) $\\lim_{z \\to -1^-} g(z)$\n",
    "(b) $\\lim_{z \\to -1^+} g(z)$\n",
    "(c) $\\lim_{z \\to -1} g(z)$"
   ]
  },
  {
   "cell_type": "markdown",
   "id": "6eb9a3f4-6d7c-421f-8d00-b082e76a1bbc",
   "metadata": {},
   "source": [
    "---\n",
    "\n",
    "### **Solutions**\n",
    "\n",
    "For  \n",
    "$$\n",
    "g(z) = \\frac{z+3}{(z+1)^2}.\n",
    "$$\n",
    "\n",
    "#### (a) $\\lim_{z \\to -1^-} g(z)$\n",
    "\n",
    "As $z \\to -1^-$ we know $z < -1$.\n",
    "\n",
    "- Numerator: $z+3 \\to 2$ (positive).  \n",
    "- Denominator: $(z+1)^2 \\to 0$ but since it’s squared, it is **always positive**.  \n",
    "  Thus,\n",
    "  $$\n",
    "  (z+1)^2 \\to 0^+.\n",
    "  $$\n",
    "\n",
    "Therefore, positive numerator over very small positive denominator gives $+\\infty$:\n",
    "$$\n",
    "\\lim_{z \\to -1^-} \\frac{z+3}{(z+1)^2} = +\\infty\n",
    "$$\n",
    "\n",
    "So,\n",
    "$$\n",
    "\\boxed{\\lim_{z \\to -1^-} g(z) = +\\infty}\n",
    "$$\n",
    "\n",
    "\n",
    "#### (b) $\\lim_{z \\to -1^+} g(z)$\n",
    "\n",
    "As $z \\to -1^+$ we know $z > -1$.\n",
    "\n",
    "- Numerator: $z+3 \\to 2$ (positive).  \n",
    "- Denominator: $(z+1)^2 \\to 0$ but again squared, so it’s **positive**.  \n",
    "  Thus,\n",
    "  $$\n",
    "  (z+1)^2 \\to 0^+.\n",
    "  $$\n",
    "\n",
    "Therefore, positive numerator over very small positive denominator gives $+\\infty$:\n",
    "$$\n",
    "\\lim_{z \\to -1^+} \\frac{z+3}{(z+1)^2} = +\\infty\n",
    "$$\n",
    "\n",
    "So,\n",
    "$$\n",
    "\\boxed{\\lim_{z \\to -1^+} g(z) = +\\infty}\n",
    "$$\n",
    "\n",
    "\n",
    "#### (c) $\\lim_{z \\to -1} g(z)$\n",
    "\n",
    "From above,\n",
    "$$\n",
    "\\lim_{z \\to -1^-} g(z) = +\\infty, \n",
    "\\qquad\n",
    "\\lim_{z \\to -1^+} g(z) = +\\infty\n",
    "$$\n",
    "\n",
    "Since both one-sided limits are $+\\infty$, the two-sided limit is also $+\\infty$:\n",
    "$$\n",
    "\\boxed{\\lim_{z \\to -1} g(z) = +\\infty}\n",
    "$$\n",
    "\n",
    "**Conclusion:** There is a **vertical asymptote** at $z = -1$.\n"
   ]
  }
 ],
 "metadata": {
  "kernelspec": {
   "display_name": "Python 3 (ipykernel)",
   "language": "python",
   "name": "python3"
  },
  "language_info": {
   "codemirror_mode": {
    "name": "ipython",
    "version": 3
   },
   "file_extension": ".py",
   "mimetype": "text/x-python",
   "name": "python",
   "nbconvert_exporter": "python",
   "pygments_lexer": "ipython3",
   "version": "3.12.6"
  }
 },
 "nbformat": 4,
 "nbformat_minor": 5
}
